\documentclass[12pt]{article}

\usepackage{EngReport}

\graphicspath{{Images/}}
\bibliography{Sources}
\onehalfspacing
\graphicspath{{images/}}
\geometry{letterpaper, portrait, includeheadfoot=true, hmargin=1in, vmargin=1in}

\renewcommand\thesection{(\arabic{section})}
\renewcommand\thesubsection{(\arabic{section}.\arabic{subsection})}
\renewcommand{\theequation}{\arabic{section}.\arabic{equation}}

%\fontsize{font size}{vertsize (usually 1.2x)}\selectfont

\begin{document}
\renewcommand{\familydefault}{\rmdefault}

\input{titlepage}
\input{headerfooter}

\section{Problem 2}
Let us have following matrices \textit{A} and \textit{B}:
\begin{equation}
    A = \begin{pmatrix}
        a_{11} & a_{12} \\
        a_{21} & a_{22}
    \end{pmatrix}
    \quad
    B = \begin{pmatrix}
        b_{11} & b_{12} \\
        b_{21} & b_{22}
    \end{pmatrix}
\end{equation}
Let us also have following matrix \textit{C}, which is a product of \textit{A} and \textit{B}:
\begin{equation}
    C = \begin{pmatrix}
        c_{11} & c_{12} \\
        c_{21} & c_{22}
    \end{pmatrix}
\end{equation}
We know from matrix multiplication formula $c_{ij} = \sum_k^na_{ik}b_{kj}$:
\begin{equation}
    \label{eq:cmatrix}
    \begin{split}
        c_{11} &= a_{11}b_{11} + a_{12}b_{21} \\
        c_{12} &= a_{11}b_{12} + a_{12}b_{22} \\
        c_{21} &= a_{21}b_{11} + a_{22}b_{21} \\
        c_{22} &= a_{21}b_{12} + a_{22}b_{22}
    \end{split}
\end{equation}
From formula of determinant of a 2x2 matrix:
\begin{equation}
    \begin{split}
        \det(A) &= a_{11}a_{22} - a_{12}a_{21} \\
        \det(B) &= b_{11}b_{22} - b_{12}b_{21} \\
        \det(C) &= c_{11}c_{22} - c_{12}c_{21}
    \end{split}
\end{equation}
So for us to prove that $\det(C) = \det(A)\det(B)$, we need to prove that:
\begin{equation}
        c_{11}c_{22} - c_{12}c_{21} = (a_{11}a_{22} - a_{12}a_{21})(b_{11}b_{22} - b_{12}b_{21})
\end{equation}
Substituting \ref{eq:cmatrix} into the left side of the equation and simplifying:
\begin{equation}
    \begin{split}
        (a_{11}b_{11}+a_{12}b_{21})(a_{21}b_{12}+a_{22}b_{22}) - (a_{11}b_{12}+a_{12}b_{22})(a_{21}b_{11}+a_{22}b_{21}) =\\
        =\cancel{a_{11}a_{21}b_{11}b_{12}} + a_{11}a_{22}b_{11}b_{22} + a_{12}a_{21}b_{12}b_{21} + \cancel{a_{12}a_{22}b_{21}b_{22}} \\
        - \cancel{a_{11}a_{21}b_{11}b_{12}} - a_{11}a_{22}b_{12}b_{21} - a_{12}a_{21}b_{11}b_{12} - \cancel{a_{12}a_{22}b_{21}b_{22}} = \\
        = a_{11}a_{22}b_{11}b_{22} + a_{12}a_{21}b_{12}b_{21} - a_{11}a_{22}b_{12}b_{21} - a_{12}a_{21}b_{11}b_{12} = \\
    \end{split} 
\end{equation}
Opening the brackets and simplifying right side of the equation:
\begin{equation}
    \begin{split}
        &(a_{11}a_{22} - a_{12}a_{21})(b_{11}b_{22} - b_{12}b_{21}) = \\
        &=a_{11}a_{22}b_{11}b_{22} + a_{12}a_{21}b_{12}b_{21} - a_{11}a_{22}b_{12}b_{21} - a_{12}a_{21}b_{11}b_{12}  
    \end{split}
\end{equation}
From this we can see that left side of the equation is equal to the right side of the equation, which proves that $\det(C) = \det(A)\det(B)$.
\section{Problem 3}
Let us find Wronskian of the following functions:
\begin{equation}
    \begin{split}
        f_1(x) &= \frac{1}{x} \\
        f_2(x) &= \frac{e^{-x^2/2}}{x} \\
        f_3(x) &= x-4
    \end{split}
\end{equation}
By definition of Wronskian:
\begin{equation}
    W = \begin{vmatrix}
        f_1(x) & f_2(x) & f_3(x) \\
        f_1'(x) & f_2'(x) & f_3'(x) \\
        f_1''(x) & f_2''(x) & f_3''(x)
    \end{vmatrix} = 
    \begin{vmatrix}
        \frac{1}{x} & \frac{e^{-x^2/2}}{x} & x-4 \\
        -\frac{1}{x^2} & \frac{e^{-x/2}(x+2)}{2x^2} & 1 \\
        \frac{2}{x^3} & \frac{e^{-x/2}(x^2+4x+8)}{4x^3}  & 0
    \end{vmatrix}
\end{equation}
Putting x = 1 into the Wronskian, we get:
\begin{equation}
    \begin{split}
        W(1) &= 
        \begin{vmatrix}
            1 & \frac{e^{-1/2}}{1} & -3 \\
            -1 & \frac{-3e^{-1/2}}{2} & 1 \\
            2 & \frac{-13e^{-1/2}}{4}  & 0
        \end{vmatrix} = -\frac{1}{2\sqrt{e}}        
    \end{split}
\end{equation}
\end{document}
